x

soundness.v
@@ -4,6 +4,107 @@ Require Import category.
 Require Import stlc.
 Require Import model.
 
-Theorem soundness : ∀ {C} `{CartesianClosed C} {Γ t} (e1 e2 : term Γ t),
+Fixpoint subst_cat {C} `{CartesianClosed C}
+{Γ Δ : context} (ρ : ∀ t, contains Γ t → term Δ t) {struct Γ}:
+Hom (ctx_denot Δ) (ctx_denot Γ).
+Proof.
+  destruct Γ.
+  + refine terminal_map.
+  + simpl.
+    apply f_prod.
+    2:{
+      apply tm_denot.
+      apply ρ.
+      apply var_zero.
+    }
+    - apply subst_cat.
+      intros.
+      apply ρ.
+      apply var_succ.
+      assumption.
+Defined.
+
+Lemma denot_comp :
+∀ {C} `{CartesianClosed C}
+{Γ Δ}
+{ρ : ∀ t : type, contains Γ t → term Δ t}
+{t}
+(c : contains Γ t),
+tm_denot (ρ t c) = compose (var_denot c) (subst_cat ρ).
+Proof.
+  intros.
+  induction c.
+  + simpl.
+    rewrite f_prod_comm2.
+    reflexivity.
+  + simpl.
+    rewrite compose_assoc.
+    rewrite f_prod_comm1.
+    rewrite <- IHc.
+    reflexivity.
+Qed.
+
+Lemma subst_denot:
+∀ {C} `{CartesianClosed C}
+{Γ Δ : context}
+{ρ : ∀ t, contains Γ t → term Δ t}
+{t} {e: term Γ t},
+tm_denot (subst ρ e) = compose (tm_denot e) (subst_cat ρ).
+Proof.
+  intros C HC HT HP HE HCC Γ Δ ρ t e.
+  induction e.
+  + simpl.
+    apply terminal_uniq.
+  + simpl.
+    rewrite IHe1.
+    rewrite IHe2.
+    apply prod_map_comp_distr.
+  + simpl.
+    rewrite IHe.
+    rewrite compose_assoc.
+    reflexivity.
+  + simpl.
+    rewrite IHe.
+    rewrite compose_assoc.
+    reflexivity.
+  + simpl.
+    apply denot_comp.
+  + simpl.
+    (* Set Printing Implicit. *)
+    rewrite IHe with (ρ := (λ (t : type) (H : contains (context_cons t1 Γ) t), exts ρ H)).
+   admit.
+  + simpl.
+    rewrite IHe1.
+    rewrite IHe2.
+    rewrite compose_assoc.
+    f_equal.
+    apply prod_map_comp_distr.
+Admitted.
+
+Theorem soundness : ∀ {C} `{CartesianClosed C} {Γ t} {e1 e2 : term Γ t},
     eqn_in_context e1 e2 → tm_denot e1 = tm_denot e2.
+Proof.
+  intros C Hc Ht Hp He Hcc Γ t e1 e2 Heq.
+  induction Heq.
+  + reflexivity.
+  + rewrite IHHeq.
+    reflexivity.
+  + rewrite IHHeq1.
+    apply IHHeq2.
+  + simpl.
+    rewrite IHHeq1.
+    rewrite IHHeq2.
+    reflexivity.
+  + simpl.
+    rewrite IHHeq.
+    reflexivity.
+  + unfold app.
+    simpl.
+   admit.
+  + admit.
+  + apply f_prod_comm1.
+  + apply f_prod_comm2.
+  + simpl.
+    symmetry.
+    apply f_prod_uniq; reflexivity.
 Admitted.
